\documentclass{article}
\usepackage{ifthen}
\usepackage{epsfig}
\usepackage[utf8]{inputenc}
\usepackage{xcolor}
\color{white}
\pagecolor{black}
\usepackage{newunicodechar}
  \makeatletter
    \def\doxynewunicodechar#1#2{%
    \@tempswafalse
    \edef\nuc@tempa{\detokenize{#1}}%
    \if\relax\nuc@tempa\relax
      \nuc@emptyargerr
    \else
      \edef\@tempb{\expandafter\@car\nuc@tempa\@nil}%
      \nuc@check
      \if@tempswa
        \@namedef{u8:\nuc@tempa}{#2}%
      \fi
    \fi
  }
  \makeatother
  \doxynewunicodechar{⁻}{${}^{-}$}% Superscript minus
  \doxynewunicodechar{²}{${}^{2}$}% Superscript two
  \doxynewunicodechar{³}{${}^{3}$}% Superscript three

\pagestyle{empty}
\begin{document}
$ x^Ty $
\pagebreak

$ |a_i| $
\pagebreak

$ 1/a_i $
\pagebreak

$ \bar{a_i} $
\pagebreak

$ e $
\pagebreak

$ e^{a_i} $
\pagebreak

$ \ln({a_i}) $
\pagebreak

$ \ln({1+a_i}) $
\pagebreak

$ \log_{10}({a_i}) $
\pagebreak

$ a_i ^ {b_i} $
\pagebreak

$ \sqrt a_i $
\pagebreak

$ 1/{\sqrt a_i} $
\pagebreak

$ a_i^2 $
\pagebreak

$ a_i^3 $
\pagebreak

$ |a_i|^2 $
\pagebreak

$ \sin^{-1} a_i $
\pagebreak

$ \cos^{-1} a_i $
\pagebreak

$ \tan^{-1} a_i $
\pagebreak

$ \gamma(a_i,x_i)= \frac{1}{|a_i|} \int_{0}^{x_i}e^{\text{-}t} t^{a_i-1} \mathrm{d} t $
\pagebreak

$ \Gamma(a_i,x_i) = \frac{1}{|a_i|} \int_{x_i}^{\infty}e^{\text{-}t} t^{a_i-1} \mathrm{d} t $
\pagebreak

$ \zeta(a_i,b_i)=\sum_{k=0}^{\infty}(b_i+k)^{\text{-}a_i} $
\pagebreak

\[ \begin{bmatrix}
    1 & 8 & 4 & 2 \\
    2 & 1 & 8 & 4 \\
    4 & 2 & 1 & 8 \\
    8 & 4 & 2 & 1
\end{bmatrix} \]
\pagebreak

$ A^T A $
\pagebreak

$ C.noalias() += \alpha op1(A) op2(B) $
\pagebreak

\[ \begin{bmatrix} 
    1 & 8 & 4 & 2 \\ 
    2 & 1 & 8 & 4 \\
    4 & 2 & 1 & 8 \\
    8 & 4 & 2 & 1
\end{bmatrix} \]
\pagebreak

$ M_2 := L_1^{-1} M_2 $
\pagebreak

$ M_3 := {L_1^*}^{-1} M_3 $
\pagebreak

$ M_4 := M_4 U_1^{-1} $
\pagebreak

$ upper(M_1) \mathrel{{+}{=}} s_1 M_2 M_2^* $
\pagebreak

$ lower(M_1) \mathbin{{-}{=}} M_2^* M_2 $
\pagebreak

$ M \mathrel{{+}{=}} s u v^* + s v u^* $
\pagebreak

$ M_2 := M_1^{-1} M_2 $
\pagebreak

\[
v =
\begin{bmatrix}
  1 \\
  2 \\
  3
\end{bmatrix}.
\]
\pagebreak

\[
A = \begin{bmatrix}
8 & 2 & 2 & 9 \\
9 & 1 & 4 & 4 \\
3 & 5 & 4 & 5
\end{bmatrix}.
\]
\pagebreak

$ A $
\pagebreak

$ A^* $
\pagebreak

$ v^* A v > 0 $
\pagebreak

$ v $
\pagebreak

$ v^* A v < 0 $
\pagebreak

$ v^* A v \ge 0 $
\pagebreak

$ v^* A v \le 0 $
\pagebreak

$ J = \bigl[ \begin{smallmatrix} O & I \\ I & O \end{smallmatrix} \bigr] $
\pagebreak

$ \bigl[ \begin{smallmatrix} 0 & 1 \\ 1 & 0 \end{smallmatrix} \bigr] $
\pagebreak

$ \mathbf{p} \equiv \mathbf{p}-0 $
\pagebreak

\[ Ax \: = \: b \]
\pagebreak

$ a^T $
\pagebreak

$ \bar{a} $
\pagebreak

$ a^* $
\pagebreak

$ a $
\pagebreak

$\ell^2$
\pagebreak

$\ell^p$
\pagebreak

$\ell^\infty$
\pagebreak

$\infty$
\pagebreak

\[
\mbox{m} = \begin{bmatrix} 1 & 2 & 6 & 9 \\
                    3 & 1 & 7 & 2 \end{bmatrix}
\]
\pagebreak

\[
\mbox{m.colwise().sum()} = \begin{bmatrix} 4 & 3 & 13 & 11 \end{bmatrix}
\]
\pagebreak

\[
\begin{bmatrix} 1 & 2 & 6 & 9 \\ 3 & 1 & 7 & 2 \end{bmatrix}
+ \begin{bmatrix} 0 & 0 & 0 & 0 \\ 1 & 1 & 1 & 1 \end{bmatrix}
= \begin{bmatrix} 1 & 2 & 6 & 9 \\ 4 & 2 & 8 & 3 \end{bmatrix}.
\]
\pagebreak

\[
  \mbox{m.colwise() - v} = 
  \begin{bmatrix}
    -1 & 21 & 4 & 7 \\
     0 & 8  & 4 & -1
  \end{bmatrix}
\]
\pagebreak

\[
  \mbox{(m.colwise() - v).colwise().squaredNorm()} =
  \begin{bmatrix}
     1 & 505 & 32 & 50
  \end{bmatrix}
\]
\pagebreak

$ \Delta u = 0 $
\pagebreak

$ Ax=b $
\pagebreak

$ x $
\pagebreak

$ b $
\pagebreak

$ m \times m $
\pagebreak

$ A^T + A $
\pagebreak

$ A^T $
\pagebreak

$ A =  P^TLDL^*P $
\pagebreak

$ A x = b $
\pagebreak

$ A = P^T L D L^* P $
\pagebreak

$ P^T y_1 = b $
\pagebreak

$ L y_2 = y_1 $
\pagebreak

$ D y_3 = y_2 $
\pagebreak

$ L^* y_4 = y_3 $
\pagebreak

$ P x = y_4 $
\pagebreak

$ D $
\pagebreak

$ \ell^p $
\pagebreak

$ \ell^\infty $
\pagebreak

$ w $
\pagebreak

$ p $
\pagebreak

\[ \Vert v - w \Vert \leqslant p\,\min(\Vert v\Vert, \Vert w\Vert). \]
\pagebreak

\[ \Vert v \Vert \leqslant p\,\vert x\vert. \]
\pagebreak

\[ \Vert v \Vert \leqslant p\,\Vert w\Vert. \]
\pagebreak

$ \sigma $
\pagebreak

$ P_\sigma $
\pagebreak

$ (e_1,\ldots,e_p) $
\pagebreak

\[ P_\sigma(e_i) = e_{\sigma(i)}. \]
\pagebreak

$ \sigma, \tau $
\pagebreak

\[ P_{\sigma\circ\tau} = P_\sigma P_\tau. \]
\pagebreak

$(ij)$
\pagebreak

$ this = this + \alpha u v^* + conj(\alpha) v u^* $
\pagebreak

$ this = this + \alpha ( u u^* ) $
\pagebreak

$ this = this + \alpha ( u^* u ) $
\pagebreak

$ s \Vert \frac{*this}{s} \Vert $
\pagebreak

$[T_{n-1} \ldots T_{i} \ldots T_{0}]$
\pagebreak

$ T_{i} $
\pagebreak

$ T_{i} M$
\pagebreak

$ M T_{i}$
\pagebreak

$ Ax = \lambda B x $
\pagebreak

$ ABx = \lambda x $
\pagebreak

$ BAx = \lambda x $
\pagebreak

$ \lambda $
\pagebreak

$ Av = \lambda v
$
\pagebreak

$ V $
\pagebreak

$ A V = V D $
\pagebreak

$ A = V D V^{-1}
$
\pagebreak

$ k $
\pagebreak

$ k
$
\pagebreak

$ A = V D
V^{-1} $
\pagebreak

$ O(n^3) $
\pagebreak

$ n $
\pagebreak

$ A = U T U^*$
\pagebreak

$25n^3$
\pagebreak

$10n^3$
\pagebreak

$ Av = \lambda v $
\pagebreak

$ A V =
V D $
\pagebreak

$ A = V D V^{-1} $
\pagebreak

$ D
$
\pagebreak

\[ \begin{bmatrix} u & v \\ -v & u \end{bmatrix} \]
\pagebreak

$ u $
\pagebreak

$ u \pm iv $
\pagebreak

$ AV = VD $
\pagebreak

$ \begin{bmatrix} u & v \\ -v & u \end{bmatrix} $
\pagebreak

$ 25n^3 $
\pagebreak

$ 10n^3 $
\pagebreak

$ B $
\pagebreak

$ Av = \lambda Bv $
\pagebreak

$ A V =
B V D $
\pagebreak

$ A = B V D V^{-1} $
\pagebreak

$ \alpha $
\pagebreak

$ \beta $
\pagebreak

$ \lambda_i = \alpha_i / \beta_i $
\pagebreak

$ \beta_i $
\pagebreak

$ \mu = \beta_i / \alpha_i$
\pagebreak

$ \mu_i A v_i = B v_i $
\pagebreak

$ \mu_i u_i^T A  = u_i^T B $
\pagebreak

$ u_i $
\pagebreak

$ x^* B x = 1 $
\pagebreak

$ B = LL^* $
\pagebreak

$ L^{-1} A (L^*)^{-1} $
\pagebreak

$ L^{*} A L $
\pagebreak

$ L^{-1} A (L^*)^{-1} (L^* x) = \lambda (L^* x) $
\pagebreak

$ Q $
\pagebreak

$ H $
\pagebreak

$ A = Q H
Q^T $
\pagebreak

$ Q^{-1} = Q^T $
\pagebreak

$ A = Q H Q^* $
\pagebreak

$ Q^{-1} = Q^* $
\pagebreak

$ 10n^3/3 $
\pagebreak

$ Q = H_{N-1} \ldots H_1 H_0 $
\pagebreak

$ H_i $
\pagebreak

$ H_i = (I - h_i v_i v_i^T) $
\pagebreak

$ h_i $
\pagebreak

$ i $
\pagebreak

$ v_i $
\pagebreak

$ v_i = [ 0, \ldots, 0, 1, M(i+2,i), \ldots, M(N-1,i) ]^T $
\pagebreak

\[ \|A\|_2 = \max_x \frac{\|Ax\|_2}{\|x\|_2} \]
\pagebreak

$ A^*A $
\pagebreak

$ A = Q S Z $
\pagebreak

$ B = Q T Z $
\pagebreak

$ U^{-1} = U^T $
\pagebreak

$ A - z B $
\pagebreak

$ A = U T U^T $
\pagebreak

$ 9n^3 $
\pagebreak

$ 4n^3/3 $
\pagebreak

$ A^{1/2} = V D^{1/2} V^{-1} $
\pagebreak

$ V D^{-1/2} V^{-1} $
\pagebreak

$ A = Q T Q^* $
\pagebreak

$ T $
\pagebreak

$ mat = Q T Q^* $
\pagebreak

$ n \cdot x + d = 0 $
\pagebreak

$ d $
\pagebreak

$ c_0*x_0 + ... + c_{d-1}*x_{d-1} + c_d = 0 $
\pagebreak

$ (\mathbf{a}+i\mathbf{b}) \times (\mathbf{c}+i\mathbf{d}) = (\mathbf{a} \times \mathbf{c} - \mathbf{b} \times \mathbf{d}) - i(\mathbf{a} \times \mathbf{d} - \mathbf{b} \times \mathbf{c})$
\pagebreak

$ \mathbf{o} $
\pagebreak

$ \mathbf{d} $
\pagebreak

$ l(t) = \mathbf{o} + t \mathbf{d} $
\pagebreak

$ t \in \mathbf{R} $
\pagebreak

$ w+xi+yj+zk $
\pagebreak

$ \left( \begin{array}{cc}
 linear & translation\\
 0 ... 0 & 1
 \end{array} \right) $
\pagebreak

$ \left( \begin{array}{cc}
 I & t \\
 0\,...\,0 & 1
 \end{array} \right) $
\pagebreak

$ \left( \begin{array}{cc}
 R & 0\\
 0\,...\,0 & 1
 \end{array} \right) $
\pagebreak

$ \left( \begin{array}{cc}
 S & 0\\
 0\,...\,0 & 1
 \end{array} \right) $
\pagebreak

$ \left( \begin{array}{c}
 v\\
 1
 \end{array} \right) $
\pagebreak

$ \left( \begin{array}{ccc}
 v_1 & ... & v_n\\
 1 & ... & 1
 \end{array} \right) $
\pagebreak

$ c, \mathbf{R}, $
\pagebreak

$ \mathbf{t} $
\pagebreak

\begin{align*}
  \frac{1}{n} \sum_{i=1}^n \vert\vert y_i - (c\mathbf{R}x_i + \mathbf{t}) \vert\vert_2^2
\end{align*}
\pagebreak

$ \Sigma_{\mathbf{x}\mathbf{y}} \in \mathbb{R}^{d \times d} $
\pagebreak

$ \mathbf{x} $
\pagebreak

$ \mathbf{y} $
\pagebreak

$d$
\pagebreak

$O(d^3)$
\pagebreak

$O(dm)$
\pagebreak

$d \times m$
\pagebreak

$ \mathbf{x} = \left( x_1, \hdots, x_n \right) $
\pagebreak

$ \mathbf{y} = \left( y_1, \hdots, y_n \right) $
\pagebreak

$ c=1 $
\pagebreak

\begin{align*}
  T = \begin{bmatrix} c\mathbf{R} & \mathbf{t} \\ \mathbf{0} & 1 \end{bmatrix}
\end{align*}
\pagebreak

$ H *this = [ beta 0 ... 0]^T $
\pagebreak

$ H = I - tau v v^*$
\pagebreak

$ v^T = [1 essential^T] $
\pagebreak

$ n \times n $
\pagebreak

$ H = \prod_{i=0}^{n-1} H_i $
\pagebreak

$ H_i = I - h_i v_i
v_i^* $
\pagebreak

$
v_i $
\pagebreak

\[ 
v_i = [\underbrace{0, \ldots, 0}_{i-1\mbox{ zeros}}, 1, \underbrace{*, \ldots,*}_{n-i\mbox{ arbitrary entries}} ]. 
\]
\pagebreak

$ n-i $
\pagebreak

$ MH $
\pagebreak

$ M $
\pagebreak

$ HM $
\pagebreak

$ H = H_0 H_1 \ldots H_{n-1} $
\pagebreak

$ H = H_{\mathrm{shift}}
H_{\mathrm{shift}+1} \ldots H_{n-1} $
\pagebreak

$ H^T = H_{n-1}^T \ldots H_1^T H_0^T $
\pagebreak

$ S P A P' S \approx L L' $
\pagebreak

$ B = S P A P' S $
\pagebreak

$ \beta > 0 $
\pagebreak

$ B + (\sigma+|\beta| I $
\pagebreak

$ \sigma = 10^{-3} $
\pagebreak

$ \theta $
\pagebreak

$ J = \left ( \begin{array}{cc} c & \overline s \\ -s  & \overline c \end{array} \right ) $
\pagebreak

$ v = J^* v $
\pagebreak

$ B = \left ( \begin{array}{cc} x & y \\ \overline y & z \end{array} \right )$
\pagebreak

$ A = J^* B J $
\pagebreak

$ B = \left ( \begin{array}{cc} \text{this}_{pp} & \text{this}_{pq} \\ (\text{this}_{pq})^* & \text{this}_{qq} \end{array} \right )$
\pagebreak

$ G^* $
\pagebreak

$ V = \left ( \begin{array}{c} p \\ q \end{array} \right )$
\pagebreak

$ G^* V = \left ( \begin{array}{c} r \\ 0 \end{array} \right )$
\pagebreak

$ B = \left ( \begin{array}{cc} \text{*this.row}(p) \\ \text{*this.row}(q) \end{array} \right ) $
\pagebreak

$ B = \left ( \begin{array}{cc} \text{*this.col}(p) & \text{*this.col}(q) \end{array} \right ) $
\pagebreak

$ \left ( \begin{array}{cc} x \\ y \end{array} \right )  =  J \left ( \begin{array}{cc} x \\ y \end{array} \right ) $
\pagebreak

$ A = P^{-1} L U Q^{-1} $
\pagebreak

$ P^{-1} L U Q^{-1} $
\pagebreak

$ \vert pivot \vert \leqslant threshold \times \vert maxpivot \vert $
\pagebreak

\[
 \mathbf{A} \, \mathbf{P} = \mathbf{Q} \, \mathbf{R}
\]
\pagebreak

\[
 \mathbf{A} \, \mathbf{P} = \mathbf{Q} \,
                    \begin{bmatrix} \mathbf{T} &  \mathbf{0} \\
                                    \mathbf{0} & \mathbf{0} \end{bmatrix} \, \mathbf{Z}
\]
\pagebreak

\[\mathrm{minimize} \|A X - B\|, \]
\pagebreak

$ \mathbf{Z}^* * \mathbf{rhs} $
\pagebreak

\[
 \mathbf{P} \, \mathbf{A} \, \mathbf{P}' = \mathbf{Q} \, \mathbf{R}
\]
\pagebreak

\[
 \mathbf{A} = \mathbf{Q} \, \mathbf{R}
\]
\pagebreak

$ P_r $
\pagebreak

$P_r A P_c^T = L U$
\pagebreak

$ P_c^T $
\pagebreak

$ A X = B $
\pagebreak

\[ A = U S V^* \]
\pagebreak

$ O(n^2p) $
\pagebreak

$ \vert singular value \vert \leqslant threshold \times \vert max singular value \vert $
\pagebreak

$ \Vert A x - b \Vert $
\pagebreak

$ A V = D V $
\pagebreak

$ A V = D B V $
\pagebreak

$ CINV = (C * C^T)^{-1} * C $
\pagebreak

$ 1/2((Ax).x) - bx $
\pagebreak

$ Cx \le f $
\pagebreak

$ 2^{-s} $
\pagebreak

$ (V+U)(V-U)^{-1} $
\pagebreak

$ \exp(A) $
\pagebreak

$ A = 0 $
\pagebreak

$ s $
\pagebreak

$ 2^{-s} x $
\pagebreak

$ \exp(2^{-\mbox{squarings}}M) $
\pagebreak

$ M = 0 $
\pagebreak

\[ 
    \sum_{k=i}^m A_{ik} X_{kj} + \sum_{k=1}^j X_{ik} B_{kj} = C_{ij}. 
\]
\pagebreak

\[ 
    X_{ij} = \frac{1}{A_{ii} + B_{jj}} \Bigl( C_{ij}
    - \sum_{k=i+1}^m A_{ik} X_{kj} - \sum_{k=1}^{j-1} X_{ik} B_{kj} \Bigr).
\]
\pagebreak

$ i=m,\ldots,1 $
\pagebreak

$ j=1,\ldots,n $
\pagebreak

$ (-1, 1) $
\pagebreak

$ A^p $
\pagebreak

$
\exp(p \log(A)) $
\pagebreak

$ 1 + 3x^2 $
\pagebreak

$ [ 1, 0, 3 ] $
\pagebreak

$ |x| \le 1 $
\pagebreak

$ 3 + x^2 $
\pagebreak

$ [ 3, 0, 1 ] $
\pagebreak

\begin{align*}
  C(u) & = \sum_{i=0}^{n}N_{i,p}(u)P_i
\end{align*}
\pagebreak

$u$
\pagebreak

\begin{align*}
  C(u) & = \sum_{i=0}^{n}N_{i,p}P_i
\end{align*}
\pagebreak

$u \in [0;1]$
\pagebreak

\begin{align*}
  \frac{d^i}{du^i}C(u) & = \sum_{i=0}^{n} \frac{d^i}{du^i} N_{i,p}(u)P_i
\end{align*}
\pagebreak

$p+1$
\pagebreak

$P_i$
\pagebreak

$p$
\pagebreak

\begin{align*}
  N_{i,p}(u), \hdots, N_{i+p+1,p}(u)
\end{align*}
\pagebreak

\begin{align*}
  \frac{d^i}{du^i} N_{i,p}(u), \hdots, \frac{d^i}{du^i} N_{i+p+1,p}(u)
\end{align*}
\pagebreak

\begin{align*}
 u_0 & = \hdots = u_p = 0 \\
 u_{m-p} & = \hdots = u_{m} = 1 \\
 u_{j+p} & = \frac{1}{p}\sum_{i=j}^{j+p-1}\bar{u}_i \quad\quad j=1,\hdots,n-p
\end{align*}
\pagebreak

$m+1$
\pagebreak

\end{document}
